{
 "cells": [
  {
   "cell_type": "markdown",
   "metadata": {},
   "source": [
    "Sure, here's the derivation of the least squares estimator for $\\beta_1$ in LaTeX:\n",
    "\n",
    "Let's start with the population regression function:\n",
    "\n",
    "\\begin{equation}\n",
    "Y = \\beta_0 + \\beta_1 X + u\n",
    "\\end{equation}\n",
    "\n",
    "The least squares estimator for $\\beta_1$ is given by:\n",
    "\n",
    "$b_1 = (\\bar{Y} - b_2 \\bar{X})$\n",
    "\n",
    "\\begin{equation}\n",
    "\\hat{\\beta}_1 = \\frac{\\sum_{i=1}^{n} (X_i - \\bar{X})(Y_i - \\bar{Y})}{\\sum_{i=1}^{n} (X_i - \\bar{X})^2}\n",
    "\\end{equation}\n",
    "\n",
    "To derive this, we need to minimize the sum of squared residuals:\n",
    "\n",
    "\\begin{equation}\n",
    "\\sum_{i=1}^{n} (Y_i - \\hat{Y}_i)^2 = \\sum_{i=1}^{n} (Y_i - (\\hat{\\beta}_0 + \\hat{\\beta}_1 X_i))^2\n",
    "\\end{equation}\n",
    "\n",
    "Taking the partial derivative with respect to $\\hat{\\beta}_1$, we get:\n",
    "\n",
    "\\begin{align}\n",
    "\\frac{\\partial}{\\partial \\hat{\\beta}_1} \\sum_{i=1}^{n} (Y_i - (\\hat{\\beta}_0 + \\hat{\\beta}_1 X_i))^2 &= -2 \\sum_{i=1}^{n} (Y_i - (\\hat{\\beta}_0 + \\hat{\\beta}_1 X_i))X_i \\\\\n",
    "&= -2 \\sum_{i=1}^{n} (Y_i X_i - \\hat{\\beta}_0 X_i - \\hat{\\beta}_1 X_i^2)\n",
    "\\end{align}\n",
    "\n",
    "Setting this derivative equal to zero and solving for $\\hat{\\beta}_1$, we get:\n",
    "\n",
    "\\begin{align}\n",
    "0 &= -2 \\sum_{i=1}^{n} (Y_i X_i - \\hat{\\beta}_0 X_i - \\hat{\\beta}_1 X_i^2) \\\\\n",
    "\\sum_{i=1}^{n} Y_i X_i &= \\hat{\\beta}_0 \\sum_{i=1}^{n} X_i + \\hat{\\beta}_1 \\sum_{i=1}^{n} X_i^2 \\\\\n",
    "\\hat{\\beta}_1 &= \\frac{\\sum_{i=1}^{n} (X_i - \\bar{X})(Y_i - \\bar{Y})}{\\sum_{i=1}^{n} (X_i - \\bar{X})^2}\n",
    "\\end{align}\n",
    "\n",
    "This is the derivation of the least squares estimator for $\\beta_1$ in Dougherty's \"Introduction to Econometrics\" 5th edition. Let me know if you have any further questions!"
   ]
  },
  {
   "cell_type": "markdown",
   "metadata": {},
   "source": [
    "Sure, here's the derivation of the formula for the least squares estimator of $\\beta_0$, which is $b_0 = \\bar{Y} - b_1 \\bar{X}$, in LaTeX:\n",
    "\n",
    "We start with the population regression function:\n",
    "\n",
    "\\begin{equation}\n",
    "Y = \\beta_0 + \\beta_1 X + u\n",
    "\\end{equation}\n",
    "\n",
    "The least squares estimator for $\\beta_1$ is given by:\n",
    "\n",
    "\\begin{equation}\n",
    "b_1 = \\frac{\\sum_{i=1}^{n} (X_i - \\bar{X})(Y_i - \\bar{Y})}{\\sum_{i=1}^{n} (X_i - \\bar{X})^2}\n",
    "\\end{equation}\n",
    "\n",
    "To derive the expression for $b_0$, we can rearrange the population regression function to solve for $\\beta_0$:\n",
    "\n",
    "\\begin{equation}\n",
    "Y = \\beta_0 + \\beta_1 X + u\n",
    "\\end{equation}\n",
    "\n",
    "Taking the expected value of both sides, we get:\n",
    "\n",
    "\\begin{equation}\n",
    "\\mathbb{E}[Y] = \\beta_0 + \\beta_1 \\mathbb{E}[X]\n",
    "\\end{equation}\n",
    "\n",
    "Substituting the sample means, we get:\n",
    "\n",
    "\\begin{equation}\n",
    "\\bar{Y} = \\beta_0 + \\beta_1 \\bar{X}\n",
    "\\end{equation}\n",
    "\n",
    "Rearranging this equation, we get the expression for the least squares estimator of $\\beta_0$:\n",
    "\n",
    "\\begin{equation}\n",
    "b_0 = \\bar{Y} - b_1 \\bar{X}\n",
    "\\end{equation}\n",
    "\n",
    "This is the derivation of the formula for the least squares estimator of $\\beta_0$ in Dougherty's \"Introduction to Econometrics\" 5th edition. Let me know if you have any further questions!"
   ]
  },
  {
   "cell_type": "markdown",
   "metadata": {},
   "source": [
    "Sure, here's the derivation of the formula for the least squares estimator of $\\beta_0$, which is $b_0 = \\bar{Y} - b_1 \\bar{X}$, in LaTeX:\n",
    "\n",
    "We start with the population regression function:\n",
    "\n",
    "\\begin{equation}\n",
    "Y = \\beta_0 + \\beta_1 X + u\n",
    "\\end{equation}\n",
    "\n",
    "The least squares estimator for $\\beta_1$ is given by:\n",
    "\n",
    "\\begin{equation}\n",
    "b_1 = \\frac{\\sum_{i=1}^{n} (X_i - \\bar{X})(Y_i - \\bar{Y})}{\\sum_{i=1}^{n} (X_i - \\bar{X})^2}\n",
    "\\end{equation}\n",
    "\n",
    "To derive the expression for $b_0$, we can rearrange the population regression function to solve for $\\beta_0$:\n",
    "\n",
    "\\begin{equation}\n",
    "Y = \\beta_0 + \\beta_1 X + u\n",
    "\\end{equation}\n",
    "\n",
    "Taking the expected value of both sides, we get:\n",
    "\n",
    "\\begin{equation}\n",
    "\\mathbb{E}[Y] = \\beta_0 + \\beta_1 \\mathbb{E}[X]\n",
    "\\end{equation}\n",
    "\n",
    "Substituting the sample means, we get:\n",
    "\n",
    "\\begin{equation}\n",
    "\\bar{Y} = \\beta_0 + \\beta_1 \\bar{X}\n",
    "\\end{equation}\n",
    "\n",
    "Rearranging this equation, we get the expression for the least squares estimator of $\\beta_0$:\n",
    "\n",
    "\\begin{equation}\n",
    "b_0 = \\bar{Y} - b_1 \\bar{X}\n",
    "\\end{equation}\n",
    "\n",
    "This is the derivation of the formula for the least squares estimator of $\\beta_0$ in Dougherty's \"Introduction to Econometrics\" 5th edition. Let me know if you have any further questions!"
   ]
  }
 ],
 "metadata": {
  "language_info": {
   "name": "python"
  }
 },
 "nbformat": 4,
 "nbformat_minor": 2
}
